src/arch/x64/X64.Vale.State_i.fsti
@@ -3,42 +3,15 @@ module X64.Vale.State_i
 
 open X64.Machine_s
 open X64.Vale
-open X64.Memory_i
 
-noeq type state = {
-  ok: bool;
-  regs: Regs_i.t;
-  xmms: Xmms_i.t;
-  flags: nat64;
-  mem: mem;
-}
-
-let reg_to_int (r:reg) : int =
-  match r with
-  | Rax -> 0
-  | Rbx -> 1
-  | Rcx -> 2
-  | Rdx -> 3
-  | Rsi -> 4
-  | Rdi -> 5
-  | Rbp -> 6
-  | Rsp -> 7
-  | R8 -> 8
-  | R9 -> 9
-  | R10 -> 10
-  | R11 -> 11
-  | R12 -> 12
-  | R13 -> 13
-  | R14 -> 14
-  | R15 -> 15
-
+unfold let state = X64.Machine_s.state
 
 [@va_qattr]
 unfold let eval_reg (r:reg) (s:state) : nat64 = s.regs r
 [@va_qattr]
 unfold let eval_xmm (x:xmm) (s:state) : Types_s.quad32 = s.xmms x
 [@va_qattr]
-unfold let eval_mem (ptr:int) (s:state) : GTot nat64 = load_mem64 ptr s.mem
+unfold let eval_mem (ptr:int) (s:state) : nat64 = load_mem64 ptr s.mem
 
 [@va_qattr]
 let eval_maddr (m:maddr) (s:state) : int =
@@ -53,7 +26,7 @@ let to_nat64 (i:int) : nat64 =
   if 0 <= i && i < 0x10000000000000000 then i else int_to_nat64 i
 
 [@va_qattr]
-let eval_operand (o:operand) (s:state) : GTot nat64 =
+let eval_operand (o:operand) (s:state) : nat64 =
   match o with
   | OConst n -> to_nat64 n
   | OReg r -> eval_reg r s
@@ -68,10 +41,10 @@ let update_xmm (x:xmm) (v:Types_s.quad32) (s:state) : state =
   { s with xmms = fun x' -> if x = x' then v else s.xmms x' }
 
 [@va_qattr]
-let update_mem (ptr:int) (v:nat64) (s:state) : GTot state = { s with mem = store_mem64 ptr v s.mem }
+let update_mem (ptr:int) (v:nat64) (s:state) : state = { s with mem = store_mem64 ptr v s.mem }
 
 [@va_qattr]
-let update_operand (o:operand) (v:nat64) (sM:state) : GTot state =
+let update_operand (o:operand) (v:nat64) (sM:state) : state =
   match o with
   | OConst n -> sM
   | OReg r -> update_reg r v sM
