src/arch/x64/X64.Vale.StateLemmas_i.fsti
@@ -3,55 +3,16 @@ open X64.Machine_s
 open X64.Vale.State_i
 open FStar.FunctionalExtensionality
 module S = X64.Semantics_s
-module BS = X64.Bytes_Semantics_s
-module ME = X64.Memory_i_s
-
-unfold let ok' s = s.ME.state.BS.ok
-unfold let regs' s = s.ME.state.BS.regs
-unfold let xmms' s = s.ME.state.BS.xmms
-unfold let flags' s = s.ME.state.BS.flags
-unfold let mem' = ME.Mkstate'?.mem
-
-val state_to_S : s:state -> GTot ME.state
-val state_of_S : s:ME.state -> state
-
-val lemma_to_ok : s:state -> Lemma
-  (ensures s.ok == ok' (state_to_S s))
-  [SMTPat s.ok]
-
-val lemma_to_flags : s:state -> Lemma
-  (ensures s.flags == flags' (state_to_S s))
-  [SMTPat s.flags]
-
-val lemma_to_mem : s:state -> Lemma
-  (ensures s.mem == mem' (state_to_S s))
-  [SMTPat s.mem]
-  
-val lemma_to_reg : s:state -> r:reg -> Lemma
-  (ensures s.regs r == regs' (state_to_S s) r)
-  [SMTPat (s.regs r)]
-
-val lemma_to_xmm : s:state -> x:xmm -> Lemma
-  (ensures s.xmms x == xmms' (state_to_S s) x)
-  [SMTPat (s.xmms x)]
 
 val lemma_to_eval_operand : s:state -> o:operand -> Lemma
-  (ensures eval_operand o s == S.eval_operand o (state_to_S s))
+  (ensures eval_operand o s == S.eval_operand o s)
   [SMTPat (eval_operand o s)]
 
 val lemma_to_eval_xmm : s:state -> x:xmm -> Lemma
-  (ensures eval_xmm x s == S.eval_xmm x (state_to_S s))
+  (ensures eval_xmm x s == S.eval_xmm x s)
   [SMTPat (eval_xmm x s)]
 
 val lemma_to_valid_operand : s:state -> o:operand -> Lemma
-  (ensures valid_operand o s ==> S.valid_operand o (state_to_S s))
+  (ensures valid_operand o s ==> S.valid_operand o s)
   [SMTPat (valid_operand o s)]
-
-val lemma_of_to : s:state -> Lemma
-  (ensures s == state_of_S (state_to_S s))
-  [SMTPat (state_of_S (state_to_S s))]
-
-val lemma_to_of : s:ME.state -> Lemma
-  (ensures s == state_to_S (state_of_S s))
-  [SMTPat (state_to_S (state_of_S s))]
 
